Setlec/TTVerify.lean
@@ -19,6 +19,7 @@ import Setlec.TTVerify.StrLitStep
 import Setlec.TTVerify.ProjStep
 import Setlec.TTVerify.DefEqStep
 import Setlec.TTVerify.IotaStep
+import Setlec.TTVerify.ProofIrrelStep
 import Setlec.TTVerify.Extend
 import Setlec.TTVerify.Consistency
 import Setlec.TTVerify.HasTypeSubst
